theories/typing/lib/vec/vec_slice.v
@@ -1,0 +1,75 @@
+From lrust.typing Require Export type.
+From lrust.typing Require Import uniq_array_util typing.
+From lrust.typing.lib Require Import vec.vec slice.uniq_slice.
+Set Default Proof Using "Type".
+
+Implicit Type 𝔄 𝔅: syn_type.
+
+Section vec_slice.
+  Context `{!typeG Σ}.
+
+  Definition vec_to_slice: val :=
+    fn: ["bv"] :=
+      let: "v" := !"bv" in delete [ #1; "bv"];;
+      let: "r" := new [ #2] in
+      "r" <- !"v";; "r" +ₗ #1 <- !("v" +ₗ #1);;
+      return: ["r"].
+
+  Lemma vec_to_uniq_slice_type {𝔄} (ty: type 𝔄) :
+    typed_val vec_to_slice (fn<α>(∅; &uniq{α} (vec_ty ty)) → uniq_slice α ty)
+      (λ post '-[(al, al')], length al' = length al → post (zip al al')).
+  Proof.
+    eapply type_fn; [apply _|]=>/= α ??[bv[]]. simpl_subst.
+    iIntros (?(vπ &[])?) "#LFT #TIME #PROPH UNIQ E Na L C /=[bv _] Obs".
+    rewrite tctx_hasty_val. iDestruct "bv" as ([|]) "[_ box]"=>//.
+    case bv as [[|bv|]|]=>//=. rewrite split_mt_uniq_bor.
+    iDestruct "box" as "[(#In &%&%& %ξi &>[% %Eq2]& ↦bv & Vo & Bor) †bv]".
+    wp_read. wp_seq. rewrite freeable_sz_full -heap_mapsto_vec_singleton.
+    wp_apply (wp_delete with "[$↦bv $†bv]"); [done|]. iIntros "_".
+    iMod (lctx_lft_alive_tok α with "E L") as (?) "(α & L & ToL)"; [solve_typing..|].
+    iMod (bor_acc_cons with "LFT Bor α") as "[big ToBor]"; [done|]. wp_seq.
+    iDestruct "big" as (? d') "(#⧖ & Pc & big)". rewrite split_mt_vec.
+    case d'=>// ?. iDestruct "big" as (??? aπl ->) "(↦₀ & ↦₁ & ↦₂ & ↦tys & ex & †)".
+    wp_bind (new _). iApply (wp_cumulative_time_receipt with "TIME"); [done|].
+    iApply wp_new; [done..|]. iIntros "!>" (?) "[†r ↦r] ⧗". wp_let.
+    set ξ := PrVar _ ξi. iDestruct (uniq_agree with "Vo Pc") as %[Eq1 ->].
+    have ->: vπ = λ π, (lapply aπl π, π ξ).
+    { by rewrite [vπ]surjective_pairing_fun Eq1 Eq2. }
+    rewrite !heap_mapsto_vec_cons. iDestruct "↦r" as "(↦r & ↦r' &_)".
+    wp_read. wp_write. do 2 wp_op. wp_read. wp_write. do 2 wp_seq.
+    iMod (uniq_intro_vec aπl with "PROPH UNIQ") as (ζil) "VoPcs"; [done|].
+    iDestruct (uniq_proph_tok_vec with "VoPcs") as "[ζl VoPcs]".
+    set aπζil := vzip _ _. set ζl := map _ aπζil.
+    set aπl' := vmap (λ aπζi (π: proph_asn),
+      π (PrVar (𝔄 ↾ prval_to_inh aπζi.1) aπζi.2): 𝔄) aπζil.
+    set aaπl := vmap (λ aπζi π,
+      (aπζi.1 π, π (PrVar (𝔄 ↾ prval_to_inh aπζi.1) aπζi.2): 𝔄)) aπζil.
+    iMod (uniq_preresolve ξ ζl (lapply aπl') with "PROPH Vo Pc ζl")
+      as "(Obs' & ζl & ToPc)"; [done|..].
+    { rewrite -vec_to_list_apply. apply proph_dep_constr, proph_dep_prvars. }
+    iCombine "Obs' Obs" as "#?". iSpecialize ("VoPcs" with "ζl").
+    iDestruct (big_sepL_sep with "VoPcs") as "[Vos Pcs]".
+    iMod ("ToBor" $! (big_sepL _ _) with "[⧗ ↦₀ ↦₁ ↦₂ ex † ToPc] [↦tys Pcs]")
+      as "[Bor α]"; last first.
+    - iMod ("ToL" with "α L") as "L". rewrite cctx_interp_singleton.
+      iMod (bor_big_sepL with "LFT Bor") as "Bors"; [done|].
+      iApply ("C" $! [# #_] -[lapply aaπl] with "Na L [-]").
+      + rewrite/= right_id (tctx_hasty_val #_) -freeable_sz_full. iExists _.
+        iFrame "⧖ †r". iNext. rewrite split_mt_uniq_slice. iFrame "In".
+        iExists _, _, _, _. rewrite big_sepL_sep. by iFrame.
+      + iApply proph_obs_impl; [|done]=>/= π [-> Imp].
+        have ->: lapply aaπl π = zip (lapply aπl π) (lapply aπl' π).
+        { clear. induction aπl; inv_vec ζil=>//= *. by f_equal. }
+        apply Imp. clear. induction aπl; inv_vec ζil=>//= *. by f_equal.
+    - iNext. iApply (merge_big_sepL_proph_ctrl_mt_ty_own with "[] Pcs ↦tys").
+      iApply persistent_time_receipt_mono; [|done]. lia.
+    - iIntros "!> big".
+      iDestruct (split_big_sepL_proph_ctrl_mt_ty_own with "PROPH ⧖ big") as "big".
+      iMod (bi.later_exist_except_0 with "big") as (wπl ?) "(>⧖' & Eqzs & ↦tys)".
+      iMod (cumulative_persistent_time_receipt with "TIME ⧗ ⧖'") as "⧖'"; [solve_ndisj|].
+      iIntros "!>!>". iExists (lapply wπl), _. iFrame "⧖'". iSplitL "Eqzs ToPc".
+      { iApply "ToPc". rewrite -!vec_to_list_apply.
+        iApply proph_eqz_constr. iApply (proph_eqz_prvars with "Eqzs"). }
+      rewrite split_mt_vec. iExists _, _, _, _. by iFrame.
+  Qed.
+End vec_slice.
